@prefix : <http://pid.geoscience.gov.au/def/voc/ga/igsn/registration/> .
@prefix rdfs: <http://www.w3.org/2000/01/rdf-schema#> .
@prefix xsd: <http://www.w3.org/2001/XMLSchema#> .
@prefix owl: <http://www.w3.org/2002/07/owl#> .
@prefix dct: <http://purl.org/dc/terms/> .
@prefix dc: <http://purl.org/dc/elements/1.1/> .
@prefix skos: <http://www.w3.org/2004/02/skos/core#> .
@prefix voaf: <http://purl.org/vocommons/voaf#> .


<http://pid.geoscience.gov.au/def/voc/ga/igsn/registration> a skos:ConceptScheme ;
  dct:title "IGSN Registration Types"@en ;
  dct:description """This vocabulary contains terms describing the types of things that may be registered wintin the IGSN registration system"""@en ;
	dc:creator "Nicholas Car" ;
	dct:created "2019-03-20"^^xsd:date ;
	dct:creator <http://orcid.org/0000-0002-8742-7730> ;
	dct:issued "2019-03-20"^^xsd:date ;
	dct:issued "2019-03-20"^^xsd:date ;
	dct:publisher <http://catalogue.linked.data.gov.au/org/O-000887> ;
  dc:publisher "Geoscience Australia" ;
	dct:source <https://github.com/IGSN/metadata/blob/master/description/include/registrationType.xsd> ;
	owl:versionInfo "v1.0" ;
  skos:historyNote "This vocabulary was extracted from a previous SKOS publication of the IGSN codelists at http://pid.geoscience.gov.au/def/voc/ga/igsncode to separate what that vocabulary had as multiple skos:Collections into individual vocabularies (skos:ConceptSchemes)." ;
  skos:hasTopConcept
    :PhysicalSample ,
    :SampleCollection ,
    :SamplingFeature ;
  .

:PhysicalSample a skos:Concept ;
	skos:prefLabel "Physical sample" ;
	skos:topConceptOf <http://pid.geoscience.gov.au/def/voc/ga/igsn/registration> ;
	skos:definition "A physical sample of a feature of interest, as opposed to a digital one (such as a satellite image or other photo). Physical samples are sometimes known as 'specimens'."@en ;
  dc:creator "IGSN Technical Committee" ;
  dc:contributor "Nicholas Car" ;
  dct:contributor <http://orcid.org/0000-0002-8742-7730> ;
.

:SampleCollection a skos:Concept ;
	skos:prefLabel "Sample collection" ;
	skos:topConceptOf <http://pid.geoscience.gov.au/def/voc/ga/igsn/registration> ;
	skos:definition "A set of things"@en ;
  dc:creator "IGSN Technical Committee" ;
  dc:contributor "Nicholas Car" ;
  dct:contributor <http://orcid.org/0000-0002-8742-7730> ;
.

:SamplingFeature a skos:Concept ;
	skos:prefLabel "Sampleing feature" ;
	skos:topConceptOf <http://pid.geoscience.gov.au/def/voc/ga/igsn/registration> ;
	skos:definition "A thing which links the sampling device (sensor) to the real-world feature of interest (such as lithosphere, tissue, waterbody). Could be a station,  transect, section"@en ;
  dc:creator "IGSN Technical Committee" ;
  dc:contributor "Nicholas Car" ;
  dct:contributor <http://orcid.org/0000-0002-8742-7730> ;
.
