@prefix : <http://pid.geoscience.gov.au/def/voc/ga/igsn/relation/> .
@prefix rdfs: <http://www.w3.org/2000/01/rdf-schema#> .
@prefix xsd: <http://www.w3.org/2001/XMLSchema#> .
@prefix owl: <http://www.w3.org/2002/07/owl#> .
@prefix dct: <http://purl.org/dc/terms/> .
@prefix dc: <http://purl.org/dc/elements/1.1/> .
@prefix skos: <http://www.w3.org/2004/02/skos/core#> .
@prefix voaf: <http://purl.org/vocommons/voaf#> .


<http://pid.geoscience.gov.au/def/voc/ga/igsn/access> a skos:ConceptScheme ;
  dct:title "IGSN Resource Types"@en ;
  dct:description """This vocabulary contains terms describing the .high level categorization of the kind of resource, used as the type for an attribute of IGSN-allocated resource' root element. Note that the resource element types also have child element types as separate vocabularies: Collection Type, Feature Type and Sample Type"""@en ;
	dc:creator "Nicholas Car" ;
	dct:created "2019-03-20"^^xsd:date ;
	dct:creator <http://orcid.org/0000-0002-8742-7730> ;
	dct:issued "2019-03-20"^^xsd:date ;
	dct:issued "2019-03-20"^^xsd:date ;
	dct:publisher <http://catalogue.linked.data.gov.au/org/O-000887> ;
  dc:publisher "Geoscience Australia" ;
	dct:source <https://github.com/IGSN/metadata/blob/master/description/include/resourceType.xsd> ;
	owl:versionInfo "v1.0" ;
  skos:historyNote "This vocabulary was extracted from a previous SKOS publication of the IGSN codelists at http://pid.geoscience.gov.au/def/voc/ga/igsncode to separate what that vocabulary had as multiple skos:Collections into individual vocabularies (skos:ConceptSchemes)." ;
  skos:hasTopConcept
    :Collection ,
    :Feature ,
    :Sample ,
    :Unknown
  .

:Collection a skos:Concept ;
	skos:prefLabel "Collection" ;
  skos:definition "A set of things"@en ;
	skos:topConceptOf <http://pid.geoscience.gov.au/def/voc/ga/igsn/resource> ;
	dct:creator "IGSN Technical Committee" ;
	dct:contributor "Nicholas Car" ;
  dct:contributor <http://orcid.org/0000-0002-8742-7730> ;
.

:Feature a skos:Concept ;
	skos:inScheme <http://pid.geoscience.gov.au/def/voc/ga/igsn/resource> ;
	skos:prefLabel "Feature" ;
	skos:topConceptOf <http://pid.geoscience.gov.au/def/voc/ga/igsn/resource> ;
	skos:definition "A geographical feature of the earth that is eitehr man-made or naturally-created. Natural geographical features consist of landforms and ecosystems. For example, terrain types, physical factors of the environment are natural geographical features. Conversely, human settlements or other engineered forms are considered types of artificial geographical features."@en ;
	dct:source <https://en.wikipedia.org/wiki/Geographical_feature> ;
  dct:creator "IGSN Technical Committee" ;
  dct:contributor "Nicholas Car" ;
  dct:contributor <http://orcid.org/0000-0002-8742-7730> ;
.

:Sample a skos:Concept ;
	skos:inScheme <http://pid.geoscience.gov.au/def/voc/ga/igsn/resource> ;
	skos:prefLabel "Sample" ;
	skos:topConceptOf <http://pid.geoscience.gov.au/def/voc/ga/igsn/resource> ;
	skos:definition "Sample - Feature which is intended to be representative of a FeatureOfInterest on which Observations may be made"@en ;
	dct:source <https://www.w3.org/TR/vocab-ssn/#SOSASample> ;
  dct:creator "IGSN Technical Committee" ;
  dct:contributor "Nicholas Car" ;
  dct:contributor <http://orcid.org/0000-0002-8742-7730> ;
.

:Unknown a skos:Concept ;
	skos:prefLabel "Unknown" ;
  skos:definition "The Resource Type is not known"@en ;
	skos:topConceptOf <http://pid.geoscience.gov.au/def/voc/ga/igsn/resource> ;
  dc:creator "Nicholas Car" ;
  dct:creator <http://orcid.org/0000-0002-8742-7730> ;
.
